theories/Coherence/AddParams.v
@@ -1,6 +1,6 @@
-Require Import Util CSet IL Annotation MapDefined.
-Require Import Sim.
-Require Import Invariance Delocation DelocationAlgo DelocationCorrect.
+Require Import Util CSet IL Annotation MapDefined AllInRel.
+Require Import Sim LabelsDefined Liveness.
+Require Import Coherence Invariance Delocation DelocationAlgo DelocationCorrect.
 Require Import Liveness LabelsDefined.
 
 Arguments sim S {H} S' {H0} r t _ _.
@@ -9,10 +9,10 @@ Definition addParams (s:IL.stmt) (lv:ann (set var)) : IL.stmt :=
   let additional_params := fst (computeParameters nil nil nil s lv) in
   compile nil s additional_params.
 
-Lemma addParams_correct (E:onv val) (ili:IL.stmt) lv
+Lemma addParams_correct b (E:onv val) (ili:IL.stmt) lv
   : defined_on (getAnn lv) E
-    -> live_sound Liveness.Imperative nil nil ili lv
-    -> noUnreachableCode LabelsDefined.isCalled ili
+    -> live_sound Imperative nil nil ili lv
+    -> noUnreachableCode (isCalled b) ili
     -> sim I.state F.state bot3 Sim
           (nil, E, ili)
           (nil:list F.block, E, addParams ili lv).
@@ -34,4 +34,18 @@ Proof with eauto.
     + eapply (@live_sound_compile nil nil nil)...
       eapply is_trs...
       eapply is_live...
+Qed.
+
+Lemma addParams_live b ili lv
+  (LS:live_sound Imperative nil nil ili lv)
+  (NUC:noUnreachableCode (isCalled b) ili)
+  : live_sound FunctionalAndImperative nil nil
+               (addParams ili lv) lv.
+Proof.
+  unfold addParams.
+  eapply srd_live_functional; eauto using PIR2; eauto.
+  - eapply (@live_sound_compile nil nil nil nil);
+      eauto using is_trs, is_live.
+  - eauto using trs_srd, is_trs.
+  - exploit compile_noUnreachableCode; eauto using is_trs.
 Qed.
